Start defining the coloring step and roughly state required theorems

new-backend/reg_allocScript.sml
@@ -1,5 +1,6 @@
 open HolKernel Parse boolLib bossLib miscLib
 open listTheory sptreeTheory pred_setTheory pairTheory
+open rich_listTheory
 open alistTheory
 open BasicProvers
 open word_liveTheory
@@ -7,27 +8,17 @@ open word_langTheory
 
 val _ = new_theory "reg_alloc";
 
-(*Defines the register allocator*)
+(*Defines a graph coloring algorithm*)
 
-(*Graph representation is a list of pairs (v,edgelist)
-  [
-   v1, (u1 u2 ...);
-   v2, (...);
-   ...
-  ]
-*)
-
-(*Convert live_sets to a clash graph with David's conventions
-
-First do a conversion to (numset) sptrees
-Then flatten the sets
-*)
+(*Graph representation is sptree of unit sptrees*)
+val _ = type_abbrev("sp_graph",
+  ``:(num_set) num_map``);
 
 (*Lookup edge in spgraph*)
 val lookup_g_def = Define`
-  lookup_g x y (g:num_set num_map) =
+  lookup_g x y (g:sp_graph) =
     case lookup x g of NONE => F
-                     | SOME t => y ∈ (domain t)` 
+                     | SOME t => lookup y t = SOME ()` 
 
 (*Insert an edge x->y in spgraph*)
 val dir_g_insert_def = Define`
@@ -48,30 +39,24 @@ val list_g_insert_def = Define`
   (list_g_insert x (y::ys) g =
     undir_g_insert x y (list_g_insert x ys g))`
 
-(*Every live-set should form a clique*)
+(*Every clash-set should form a clique*)
 val clique_g_insert_def = Define`
   (clique_g_insert [] g = g) ∧ 
   (clique_g_insert (x::xs) g =
     list_g_insert x xs (clique_g_insert xs g))`
 
-val live_sets_to_sp_g_def = Define`
-  (live_sets_to_sp_g [] = LN) ∧ 
-  (live_sets_to_sp_g (x::xs) =
+val clash_sets_to_sp_g_def = Define`
+  (clash_sets_to_sp_g [] = LN) ∧ 
+  (clash_sets_to_sp_g (x::xs) =
     (*I think nub probably makes it easier*)
-    let subgraph = live_sets_to_sp_g xs in
+    let subgraph = clash_sets_to_sp_g xs in
     let clashes = nub (MAP FST (toAList x)) in
     clique_g_insert clashes subgraph)`
 
-(*Convert to clash graph representation*)
-val sp_g_to_cg_def = Define`
-  sp_g_to_cg g = 
-    MAP (λx,y. x,nub (MAP FST (toAList y))) (toAList g)`
-
-val get_cg_def = Define`
-  get_cg prog = sp_g_to_cg (live_sets_to_sp_g (merge_pair(get_live_sets prog LN)))`
-
-(*Proof idea:
-  Show that livesets always appear as cliques in the graph
+(*
+  Link up coloring_satisfactory to coloring_ok
+  Proof idea:
+  Show that clash sets always appear as cliques in the graph
   and coloring_satisfactory guarantees that cliques have all
   distinct colors
 *)
@@ -91,7 +76,7 @@ val lookup_dir_g_insert_correct = prove(``
     rw[]>>fs[lookup_insert]>>
     Cases_on`x'=x`>>fs[]>>
     FULL_CASE_TAC>>
-    fs[domain_insert])
+    fs[domain_insert,lookup_insert,lookup_def])
 
 val list_g_insert_correct = prove(``
   !ls x g.
@@ -120,6 +105,351 @@ val sp_g_is_clique_def = Define`
     !x y. MEM x ls ∧ MEM y ls ∧ x ≠ y⇒
       lookup_g x y g ∧ lookup_g y x g)`
 
+(*coloring_satisfactory for sp_graphs*)
+val coloring_satisfactory_def = Define `
+  (coloring_satisfactory col (G:sp_graph) =
+  ∀v. v ∈ domain G ⇒ 
+    let edges = lookup v G in
+    case edges of NONE => F
+                | SOME edges => ∀e. e ∈ domain edges ⇒ col e ≠ col v)`
+
+val clique_g_insert_is_clique = prove(``
+  !ls g.
+  sp_g_is_clique ls (clique_g_insert ls g)``,
+  Induct>>
+  rw[clique_g_insert_def,sp_g_is_clique_def]>>
+  TRY (metis_tac[list_g_insert_correct])
+  >>
+    fs[sp_g_is_clique_def]>>
+    metis_tac[list_g_insert_correct])
+
+val clique_g_insert_preserves_clique = prove(``
+  !ls g ls'.
+  ALL_DISTINCT ls' ∧
+  sp_g_is_clique ls g ⇒ 
+  sp_g_is_clique ls (clique_g_insert ls' g)``,
+  Induct>>
+  rw[clique_g_insert_def,sp_g_is_clique_def]>>
+  metis_tac[clique_g_insert_correct])
+
+val clash_sets_clique = prove(``
+  !ls x. 
+  MEM x ls ⇒ 
+  sp_g_is_clique (nub (MAP FST (toAList x))) (clash_sets_to_sp_g ls)``,
+  Induct>>fs[clash_sets_to_sp_g_def]>>rw[]>>
+  unabbrev_all_tac>>
+  metis_tac[clique_g_insert_is_clique
+           ,clique_g_insert_preserves_clique,all_distinct_nub])
+
+val get_spg_def = Define`
+  get_spg prog live = 
+    let (hd,clash_sets) = get_clash_sets prog live in
+      (clash_sets_to_sp_g (hd::clash_sets))`
+
+val coloring_satisfactory_cliques = prove(``
+  ∀ls g (f:num->num).
+  ALL_DISTINCT ls ∧ 
+  coloring_satisfactory f g ∧ sp_g_is_clique ls g
+  ⇒ 
+  ALL_DISTINCT (MAP f ls)``,
+  Induct>>
+  fs[sp_g_is_clique_def,coloring_satisfactory_def]>>
+  rw[]
+  >-
+    (fs[MEM_MAP]>>rw[]>>
+    first_x_assum(qspecl_then [`h`,`y`] assume_tac)>>rfs[]>>
+    Cases_on`MEM y ls`>>Cases_on`h=y`>>fs[]>>
+    fs[lookup_g_def]>>EVERY_CASE_TAC>>fs[]>>
+    imp_res_tac domain_lookup>>
+    res_tac>>fs[LET_THM]>>
+    Cases_on`lookup y g`>>fs[])
+  >>
+    first_x_assum(qspecl_then [`g`,`f`] mp_tac)>>rfs[])
+
+val MEM_nub = prove(``
+  ∀ls x. MEM x ls ⇒ MEM x (nub ls)``,
+  rw[])
+
+val coloring_satisfactory_coloring_ok_alt = prove(``
+  ∀prog f live.
+  let spg = get_spg prog live in
+  coloring_satisfactory (f:num->num) spg
+  ⇒ 
+  coloring_ok_alt f prog live``,
+  rpt strip_tac>>
+  fs[LET_THM,coloring_ok_alt_def,coloring_satisfactory_def,get_spg_def]>>
+  Cases_on`get_clash_sets prog live`>>fs[]>>
+  strip_tac>>
+  qabbrev_tac `ls = q::r`>>
+  qsuff_tac `EVERY (λs. INJ f (domain s) UNIV) ls`
+  >-
+    fs[Abbr`ls`]
+  >>
+  rw[EVERY_MEM]>>
+  imp_res_tac clash_sets_clique>>
+  imp_res_tac coloring_satisfactory_cliques>>
+  pop_assum(qspec_then`f`mp_tac)>>
+  discharge_hyps
+  >- fs[coloring_satisfactory_def,LET_THM]>>
+  discharge_hyps
+  >- fs[all_distinct_nub]>>
+  fs[INJ_DEF,all_distinct_nub]>>rw[]>>
+  fs[domain_lookup]>>
+  `MEM x (MAP FST (toAList s)) ∧
+   MEM y (MAP FST (toAList s))` by 
+    (fs[MEM_MAP,EXISTS_PROD]>>
+    metis_tac[domain_lookup,MEM_MAP,EXISTS_PROD,MEM_toAList])>>
+  `ALL_DISTINCT (nub (MAP FST (toAList s)))` by 
+    metis_tac[all_distinct_nub]>>
+  fs[EL_ALL_DISTINCT_EL_EQ]>>
+  imp_res_tac MEM_nub>>
+  fs[MEM_EL]>>pop_assum (SUBST1_TAC o SYM)>>
+  simp[]>>
+  metis_tac[EL_MAP])
+
+(*Conventions of wordLang*)
+
+(*Distinguish 3 kinds of variables:
+  Evens are physical registers
+  4n+1 are allocatable registers
+  4n+3 are stack registers*)
+
+val is_stack_var_def = Define`
+  is_stack_var (n:num) = (n MOD 4 = 3)`
+val is_phy_var_def = Define`
+  is_phy_var (n:num) = (n MOD 2 = 0)`
+val is_alloc_var_def = Define`
+  is_alloc_var (n:num) = (n MOD 4 = 1)`
+
+val coloring_conventional_def = Define`
+  coloring_conventional (G:sp_graph) k col ⇔
+  let vertices = domain G in
+  ∀x. x ∈ vertices ⇒
+    if is_phy_var x then col x = x 
+    else 
+    if is_stack_var x then is_stack_var (col x)
+    else 
+    (*x must be an alloc var, although that must be proved*)
+    let y = col x in
+      if is_phy_var y then y < 2*k
+      else 
+         is_stack_var y`
+
+(*Define the coloring step:
+  Takes arguments:
+  G = spgraph (possibly augmented e.g. in coalescing),
+  k = number of registers to use,
+  prefs = num-> num list -> num (selects a color from the list)
+  nsv = next spill var
+  ls = heuristic order to color vertices,
+
+  Result: a num sptree where looking up a vertex gives its coloring
+*)
+
+val split_vertices_def = Define`
+  split_vertices G = 
+  let ls = MAP FST (toAList G) in
+    SPLITP is_alloc_var ls`
+
+(*Deletes unavailable colors by looking up the current coloring function*)
+(*k is usually small --> just use a list, eventually a bitset*)
+val remove_colors_def = Define`
+  (*No more available colors*)
+  (remove_colors (col:num num_map) ls [] = []) ∧
+  (*Some available color after checking*) 
+  (remove_colors (col:num num_map) [] k = k) ∧
+  (*Do the checks*)
+  (remove_colors col (x::xs) k =
+    let c = lookup x col in
+    case c of NONE => remove_colors col xs k
+            | SOME c => remove_colors col xs 
+                        (FILTER (λx.x ≠ c) k))`
+
+(*EVAL``remove_colors (list_insert [1;2;3] [1;1;1] LN) [1;2;3;4] [1;2;3;4]``*)
+  
+(*NOTE: If we used redundancy in the graph representations,
+ then we would use adj lists here*)
+
+(*TODO: Make monadic on the last 2 arguments*)
+val assign_color_def = Define`
+  assign_color G k prefs v nsv col = 
+  case lookup v G of
+    (*Vertex wasn't even in the graph -- ignore*)
+    NONE => (nsv,col)
+  | SOME x =>
+    let xs = MAP FST (toAList x) in
+    let k = remove_colors col xs k in
+    case k of 
+      [] => (*Spill*) (nsv+4,col) 
+    | xs => (*Choose a preferred color*) (nsv,insert v (prefs v xs) col)` 
+
+
+(*Auxiliary that colors according to the heuristic order (first list arg).
+
+  The second list arg contains all the vertices which should actually 
+  be colored. 
+  Putting this here allows me to simplify the assumptions about 
+  the heuristic list --> it does not need to generate a complete list
+
+  TODO: maybe write this slightly differently so that we get more free 
+  assumptions (e.g. just merge the two lists at the start)
+*)
+
+(*TODO: Make monadic on the last 2 argument*)
+val find_coloring_aux = Define`
+  (find_coloring_aux G k prefs [] [] nsv col = (nsv,col)) ∧ 
+  (find_coloring_aux G k prefs [] (y::ys) nsv col =
+    (nsv,col)) ∧ 
+    (*Probably need to do this:
+    case lookup y col of
+      SOME x => (nsv,col) (*Should always occur*) 
+    | NONE => ...*)
+  (find_coloring_aux G k prefs (x::xs) ys nsv col = 
+    let (nsv,col) = assign_color G k prefs x nsv col in
+      find_coloring_aux G k prefs xs ys nsv col)`
+
+(*nsv should be the "next_stack_variable" --> could either be computed directly from G or maybe passed in as it is here*) 
+val find_coloring_def = Define`
+  find_coloring (G:sp_graph) k prefs nsv ls =
+    let (others,alloc) = split_vertices G in
+    (*Everything that cannot be alloced is identity colored*)
+    let pre_color = FOLDR (λx y. insert x x y) LN others in
+    let colors = GENLIST (λx:num.2*x) k in 
+    find_coloring_aux G colors prefs ls alloc nsv pre_color`
+
+(*Extract a coloring function from the generated sptree*)
+val total_color_def = Define`
+  total_color col = 
+    (λx. case lookup x col of NONE => x | SOME x => x)`
+
+(*VERY rough statement of the two theorems that must be proved 
+  about find_coloring. Missing many assumptions:
+  e.g. prefs must only select something from its input list
+  *)
+val find_coloring_conventional = store_thm ("find_coloring_conventional",``
+  ∀G k prefs nsv ls.
+  let (nsv',col) = find_coloring G k prefs nsv ls in
+  let col = total_color col in 
+  coloring_conventional G k col``,cheat); 
+
+val find_coloring_satisfactory = store_thm ("find_coloring_satisfactory",``
+  ∀G k prefs nsv ls.
+  let (nsv',col) = find_coloring G k prefs nsv ls in
+  let col = total_color col in
+  coloring_satisfactory col G``,cheat);
+
+(*
+(*Simplify
+  Takes a graph G,
+  The current working degree list deg_list,
+  The number of colors k
+
+  Returns a tuple (remaining vertices,stack)
+*)
+
+(*SPLITP in rich_listTheory doesn't have many theories with it
+  split_deg splits list into those less than degree and those >=
+*)
+
+val split_deg_def = Define`
+  split_deg k ls = SPLITP (λx,y:num. y<k) ls` 
+
+(*EVAL ``split_deg 2 [1,2;2,3;3,1]``*) 
+
+val decrement_def = Define`
+  (decrement (es:num_set) [] = []) ∧ 
+  (decrement es ((v,deg:num)::xs) =
+    let rest = decrement es xs in 
+    if lookup v es = SOME () then (v,deg-1)::rest else (v,deg)::rest)`
+
+val dec_deg_def = Define`
+  (dec_deg G [] ls = []) ∧ 
+  (dec_deg G (x::xs) ls) =
+    let es = lookup x G in
+    case es of NONE => dec_deg G xs ls
+            |  SOME es => dec_deg G xs (decrement es ls)`
+
+(*Single step simplification*)
+val simplify_def = Define `
+  simplify k G deg_list =
+  let (non_simp,simp) = split_deg k deg_list in
+    case simp of 
+      [] => (non_simp,[])
+    | simp => 
+      let simp = MAP FST simp in (*Discard degree information*)
+      (dec_deg G simp non_simp,simp)`
+
+(*Single step spill, arbitrarily pick x to be spilled for now*)
+val spill_def = Define `
+  spill ((x,y)::xs) = (x,xs)`
+
+(*Main loop that calls the steps WITH the recursion builtin:
+  Result should be a stack*)
+val reg_alloc_loop_def = tDefine "reg_alloc_loop" `
+  (reg_alloc_loop k G [] stack = stack) ∧ 
+  (reg_alloc_loop k G deglist stack =
+    let (deglist,newstack) = simplify k G deglist in
+    case newstack of
+      [] => (*Spilling*)
+      let (v,deglist) = spill deglist in
+        reg_alloc_loop k G deglist (v::stack)
+    | xs => reg_alloc_loop k G deglist (xs++stack))` cheat
+
+
+(*TODO:WF_REL_TAC on the size of deg_list
+  WF_REL_TAC `measure LENGTH`*)
+
+(*EVAL ``is_stack_var 7``*)
+
+(*Generate list of vertices and associated degree from spgraph
+  NOTE: 
+  1) only need to do  registers
+  2) Ignore stack registers in degree counts
+*)
+val gen_worklist_aux_def = Define`
+  (gen_worklist_aux [] = []) ∧
+  (gen_worklist_aux ((v,es)::xs) =
+    let rest = gen_worklist_aux xs in
+    if is_alloc_var v then
+      let edges = FILTER (λv. ¬ (is_stack_var v)) (MAP FST (toAList es)) in  
+      (v,LENGTH edges)::rest
+    else rest)`
+
+val gen_worklist_def = Define`
+  gen_worklist (G:sp_graph) =
+  gen_worklist_aux (toAList G)` 
+
+EVAL ``gen_worklist (get_spg
+  (Seq (Move [1,2;3,4;5,6]) 
+  (Call (SOME (3, list_insert [1;3;5;7;9] [();();();();()] LN,Skip)) (SOME 400) [7;9] NONE)) LN)``
+
+
+(*Graph representation is a list of pairs (v,edgelist)
+  Graph is undirected
+  [
+   v1, (u1 u2 ...);
+   v2, (...);
+   ...
+  ]
+*)
+
+(*Convert clash_sets to a clash graph with David's conventions
+
+First do a conversion to (numset) sptrees
+Then flatten the sets
+*)
+
+(*Convert to clash graph representation*)
+val sp_g_to_cg_def = Define`
+  sp_g_to_cg g = 
+    MAP (λx,y. x,nub (MAP FST (toAList y))) (toAList g)`
+
+val get_cg_def = Define`
+  get_cg prog live = 
+    let (hd,clash_sets) = get_clash_sets prog live in
+      sp_g_to_cg (clash_sets_to_sp_g (hd::clash_sets))`
+
+
 (*Cliques in cg*)
 val cg_is_clique_def = Define`
   (cg_is_clique ls g = 
@@ -145,41 +475,8 @@ val sp_clique_to_cg_clique = prove(``
   fs[ALOOKUP_toAList,MEM_MAP,MEM_toAList,EXISTS_PROD]>>
   metis_tac[num_set_domain,MEM_MAP])
 
-val clique_g_insert_is_clique = prove(``
-  !ls g.
-  sp_g_is_clique ls (clique_g_insert ls g)``,
-  Induct>>
-  rw[clique_g_insert_def,sp_g_is_clique_def]>>
-  TRY (metis_tac[list_g_insert_correct])
-  >>
-    fs[sp_g_is_clique_def]>>
-    metis_tac[list_g_insert_correct])
-
-val clique_g_insert_preserves_clique = prove(``
-  !ls g ls'.
-  ALL_DISTINCT ls' ∧
-  sp_g_is_clique ls g ⇒ 
-  sp_g_is_clique ls (clique_g_insert ls' g)``,
-  Induct>>
-  rw[clique_g_insert_def,sp_g_is_clique_def]>>
-  metis_tac[clique_g_insert_correct])
-
-val live_sets_clique = prove(``
-  !ls x. 
-  MEM x ls ⇒ 
-  sp_g_is_clique (nub (MAP FST (toAList x))) (live_sets_to_sp_g ls)``,
-  Induct>>fs[live_sets_to_sp_g_def]>>rw[]>>
-  unabbrev_all_tac>>
-  metis_tac[clique_g_insert_is_clique
-           ,clique_g_insert_preserves_clique,all_distinct_nub])
-
 (*Defs from David*)
 (* Coloring satisfies constraints *)
-val coloring_satisfactory_def = Define `
-    (coloring_satisfactory col [] = T) /\
-    (coloring_satisfactory col ((r, rs)::cs) = 
-      (~(MEM (col r) (MAP col rs)) ∧ (coloring_satisfactory col cs)))`
-
 val coloring_satisfactory_alt = prove(``
   !g f.
   coloring_satisfactory f g ⇒ 
@@ -204,20 +501,23 @@ val coloring_satisfactory_cliques = prove(``
   >>
     first_x_assum(qspecl_then [`g`,`f`] mp_tac)>>rfs[])
 
-val MEM_nub = prove(``
-  ∀ls x. MEM x ls ⇒ MEM x (nub ls)``,
-  rw[])
-
 val coloring_satisfactory_coloring_ok_alt = prove(``
   ∀prog f live.
-  let ls = merge_pair (get_live_sets prog live) in
-  let cg = sp_g_to_cg (live_sets_to_sp_g ls) in 
+  let cg = get_cg prog live in
   coloring_satisfactory f cg
   ⇒ 
   coloring_ok_alt f prog live``,
-  rw[coloring_ok_alt_def,coloring_satisfactory_def]>>
-  fs[EVERY_MEM,Abbr`cg`]>>rw[]>>
-  imp_res_tac live_sets_clique>>
+  rpt strip_tac>>
+  fs[LET_THM,coloring_ok_alt_def,coloring_satisfactory_def,get_cg_def]>>
+  Cases_on`get_clash_sets prog live`>>fs[]>>
+  strip_tac>>
+  qabbrev_tac `ls = q::r`>>
+  qsuff_tac `EVERY (λs. INJ f (domain s) UNIV) ls`
+  >-
+    fs[Abbr`ls`]
+  >>
+  rw[EVERY_MEM]>>
+  imp_res_tac clash_sets_clique>>
   imp_res_tac sp_clique_to_cg_clique>>
   imp_res_tac coloring_satisfactory_cliques>>
   fs[INJ_DEF,all_distinct_nub]>>rw[]>>
@@ -233,8 +533,24 @@ val coloring_satisfactory_coloring_ok_alt = prove(``
   fs[MEM_EL]>>pop_assum (SUBST1_TAC o SYM)>>
   simp[]>>
   metis_tac[EL_MAP])
+
+
+
+
+
+
+
+
+
+
+
+
+
 (* 
 EVAL ``get_cg
   (Seq (Move [1,2;3,4;5,6]) 
-  (Call (SOME (3, list_insert [1;3;5;7;9] [();();();();()] LN,Skip)) (SOME 400) [7;9] NONE))``
+  (Call (SOME (3, list_insert [1;3;5;7;9] [();();();();()] LN,Skip)) (SOME 400) [7;9] NONE)) LN``
 *)
+
+*)
+
